src/Finish/Impl.v
@@ -68,32 +68,65 @@ Section Defs.
   | PKG_END_TASK => []
   end.
 
+  Inductive pkg_parse_err :=
+  | PKG_PARSE_NOARGS_EXPECTED
+  | PKG_PARSE_TASK_EXPECTED.
+
   Structure package := make {
     pkg_task : tid;
     pkg_op: package_op;
     pkg_id: fid;
     pkg_time: nat;
     pkg_args: list nat;
-    pkg_parse_op :=
+    pkg_lineno: option nat;
+    pkg_parse :=
     match pkg_op, pkg_args with
-    | PKG_INIT, [] => Some (INIT pkg_id)
-    | PKG_BEGIN_FINISH, [] => Some (BEGIN_FINISH pkg_id)
-    | PKG_END_FINISH, [] => Some END_FINISH
-    | PKG_BEGIN_TASK, [x] => Some (BEGIN_TASK (taskid x))
-    | PKG_END_TASK, [] => Some END_TASK
-    | _, _ => None
+    | PKG_INIT, [] => inl (INIT pkg_id)
+    | PKG_BEGIN_FINISH, [] => inl (BEGIN_FINISH pkg_id)
+    | PKG_END_FINISH, [] => inl END_FINISH
+    | PKG_BEGIN_TASK, [x] => inl (BEGIN_TASK (taskid x))
+    | PKG_END_TASK, [] => inl END_TASK
+    | PKG_BEGIN_TASK, _ => inr PKG_PARSE_TASK_EXPECTED
+    | _, _ => inr PKG_PARSE_NOARGS_EXPECTED
     end;
   }.
 
   (** Test cases that catch bugs we found: *)
 
+  Goal forall p e,
+    pkg_args p <> [] ->
+    pkg_op p <> PKG_BEGIN_TASK ->
+    pkg_parse p = inr e ->
+    e = PKG_PARSE_NOARGS_EXPECTED.
+  Proof.
+    intros.
+    unfold pkg_parse in *.
+    destruct p, pkg_op0; simpl in *;
+    destruct pkg_args0; try contradiction;
+    inversion H1; subst; clear H1; trivial.
+  Qed.
+
+  Goal forall p e,
+    length (pkg_args p) <> 1 ->
+    pkg_op p = PKG_BEGIN_TASK ->
+    pkg_parse p = inr e ->
+    e = PKG_PARSE_TASK_EXPECTED.
+  Proof.
+    intros.
+    unfold pkg_parse in *.
+    destruct p, pkg_op0; simpl in *;
+    destruct pkg_args0; inversion H0; clear H0;
+    inversion H1; subst; clear H1; auto.
+    destruct pkg_args0; inversion H2; subst; auto.
+  Qed.
+
   Goal forall p n,
     pkg_args p = [n] ->
     pkg_op p = PKG_BEGIN_TASK ->
-    pkg_parse_op p = Some (BEGIN_TASK (taskid n)).
+    pkg_parse p = inl (BEGIN_TASK (taskid n)).
   Proof.
     intros.
-    unfold pkg_parse_op.
+    unfold pkg_parse.
     rewrite H0.
     rewrite H.
     trivial.
@@ -102,10 +135,10 @@ Section Defs.
   Goal forall p,
     pkg_args p = [] ->
     pkg_op p <> PKG_BEGIN_TASK ->
-    exists o, pkg_parse_op p = Some o.
+    exists o, pkg_parse p = inl o.
   Proof.
     intros.
-    unfold pkg_parse_op.
+    unfold pkg_parse.
     remember (pkg_op p).
     destruct p0; subst; rewrite H; eauto.
     contradiction.
@@ -118,23 +151,21 @@ Section Defs.
     pkg_id := (fst p);
     pkg_time := snd p;
     pkg_args := l;
+    pkg_lineno := None
   |}.
 
-  Inductive pkg_err :=
-  | PARSE_ERROR.
-
   Inductive run_err :=
-  | PKG_ERROR: pkg_err -> run_err
-  | REDUCES_ERROR: reduces_err -> run_err.
+  | RUN_PKG_PARSE_ERROR: pkg_parse_err -> run_err
+  | RUN_REDUCES_ERROR: reduces_err -> run_err.
 
   Definition run (s:state) (p:package) : (state + run_err) % type :=
-  match pkg_parse_op p with
-  | Some o =>
+  match pkg_parse p with
+  | inl o =>
     match Lang.reduces s (pkg_task p) o with
     | inl s' => inl s'
-    | inr e => inr (REDUCES_ERROR e)
+    | inr e => inr (RUN_REDUCES_ERROR e)
     end
-  | None => inr (PKG_ERROR PARSE_ERROR)
+  | inr e => inr (RUN_PKG_PARSE_ERROR e)
   end.
 
   Definition add1 s n p :=
@@ -155,12 +186,113 @@ Section Defs.
   Definition enq_cons p (e:enq) := let (x, y) := e in (x, p :: y).
 
   Definition enq_succ (e:enq) := let (x, y) := e in (S x, y).
-
+(*
   Definition enq_select p ps (e:enq) :=
   if beq_nat (enq_curr e) (pkg_time p)
   then (p::ps, enq_succ e)
   else (ps, enq_cons p e).
+*)
+  Definition enq_step (n:nat) (elems:list package) :=
+  let (l, r) :=
+    partition (fun p => beq_nat n (pkg_time p)) elems
+  in
+  (l, (if beq_nat (length l) 0 then n else (S n), r)).
 
+  Lemma partition_length:
+    forall {A : Type} (f : A -> bool) (l : list A),
+    length (fst (partition f l)) + length (snd (partition f l)) = length l.
+  Proof.
+    induction l. {
+      simpl.
+      trivial.
+    }
+    simpl.
+    remember (f a).
+    symmetry in Heqb.
+    remember (partition f l).
+    destruct p as (x, y).
+    destruct b; simpl in *;
+    auto with *.
+  Qed.
+
+  Let enq_step_length:
+    forall elems l r n,
+    enq_step n elems = (l, r) ->
+    length l + length (snd r) = length elems.
+  Proof.
+    induction elems; intros; unfold enq_step in *; simpl in *;
+    inversion H; subst; clear H.
+    - simpl.
+      trivial.
+    - remember (partition _ _).
+      remember (length elems) as z.
+      symmetry in Heqz.
+      rewrite <- partition_length with (f:=fun p : package => PeanoNat.Nat.eqb n (pkg_time p)) in Heqz.
+      rewrite <- Heqp in *.
+      remember (PeanoNat.Nat.eqb n _).
+      symmetry in Heqb.
+      destruct b. {
+        rewrite PeanoNat.Nat.eqb_eq in *.
+        rewrite Heqb in *; clear Heqb.
+        destruct p as (a1, b1).
+        remember (PeanoNat.Nat.eqb _ _).
+        symmetry in Heqb.
+        destruct b. {
+          rewrite PeanoNat.Nat.eqb_eq in *.
+          simpl in *.
+          inversion Heqb.
+        }
+        rewrite PeanoNat.Nat.eqb_neq in *.
+        inversion H1; subst; clear H1.
+        simpl.
+        trivial.
+      }
+      rewrite PeanoNat.Nat.eqb_neq in *.
+      destruct p as (a1, b1).
+      remember (PeanoNat.Nat.eqb _ _).
+      symmetry in Heqb0.
+      destruct b. {
+        rewrite PeanoNat.Nat.eqb_eq in *.
+        inversion H1; subst; clear H1.
+        simpl.
+        rewrite Heqb0.
+        simpl.
+        trivial.
+      }
+      inversion H1; subst; clear H1.
+      rewrite PeanoNat.Nat.eqb_neq in *.
+      simpl.
+      auto with *.
+  Qed.
+
+  Function enq_partition (n:nat) (elems: list package) {measure length elems} :=
+  let (l1, e1) := enq_step n elems in
+  match l1 with
+  | [] => (l1, e1)
+  | _ =>
+    let (l2, e2) := enq_partition (fst e1) (snd e1) in
+    (l1 ++ l2, e2)
+  end.
+  Proof.
+    intros.
+    apply enq_step_length in teq.
+    rewrite <- teq.
+    simpl.
+    auto with *.
+  Defined.
+
+  Goal enq_partition 0 [
+    pkg_create (taskid 0) (finishid 1, 1) PKG_BEGIN_TASK [1];
+    pkg_create (taskid 0) (finishid 1, 0) PKG_INIT []
+  ] = ([
+    pkg_create (taskid 0) (finishid 1, 0) PKG_INIT [];
+    pkg_create (taskid 0) (finishid 1, 1) PKG_BEGIN_TASK [1]
+  ], (2, [])).
+  Proof.
+    compute.
+    trivial.
+  Qed.
+(*
   Goal enq_select (pkg_create (taskid 0) (finishid 1, 0) PKG_INIT []) [] enq_zero
     = ([pkg_create (taskid 0) (finishid 1, 0) PKG_INIT []], (1, [])).
   Proof.
@@ -198,22 +330,7 @@ Section Defs.
     compute.
     trivial.
   Qed.
-
-  Fixpoint add_all (s:state) (n:nat) (elems:list package) {struct elems} : ((state + run_err) * (nat * list package)) % type:=
-  match elems with
-  | nil => (inl s, (n, nil))
-  | p::ps =>
-    match ps with
-    | nil => add1 s n p
-    | _ =>
-      let result := add_all s n ps in
-      match fst result with
-      | inl s' => add1 s' n p
-      | _ => result
-      end
-    end
-  end.
-
+*)
   Definition buffer :=  Map_FID.t enq.
 
   Structure checks := {
@@ -227,7 +344,7 @@ Section Defs.
   | Some e => e
   | None => enq_zero
   end) in
-  let (l, e) := poll_ready (fst e) (snd e) in
+  let (l, e) := enq_partition (fst e) (snd e) in
   (l, Map_FID.add f e b).
 
   Goal buffer_add (pkg_create (taskid 0) (finishid 1, 0) PKG_INIT []) (Map_FID.empty _) =
@@ -278,6 +395,51 @@ Section Defs.
     trivial.
   Qed.
 
+  Goal
+    let l := [
+      pkg_create (taskid 0) (finishid 1, 1) PKG_BEGIN_TASK [1]
+    ] in
+    let m := Map_FID.add (finishid 1) (0, l) (Map_FID.empty _) in
+    buffer_add_all l (Map_FID.empty _) = ([], m).
+  Proof.
+    compute.
+    trivial.
+  Qed.
+
+  Goal
+    let l1 := [
+      pkg_create (taskid 0) (finishid 1, 1) PKG_BEGIN_TASK [1]
+    ] in
+    let l2 := [
+      pkg_create (taskid 0) (finishid 1, 0) PKG_INIT []
+    ] in
+    let l3 := [
+      pkg_create (taskid 0) (finishid 1, 0) PKG_INIT [];
+      pkg_create (taskid 0) (finishid 1, 1) PKG_BEGIN_TASK [1]
+    ] in
+    let m := Map_FID.add (finishid 1) (0, l1) (Map_FID.empty _) in
+    buffer_add_all l2 m = (l3, Map_FID.add (finishid 1) (2, []) m).
+  Proof.
+    intros.
+    compute.
+    trivial.
+  Qed.
+
+  Goal
+    let l := [
+      pkg_create (taskid 0) (finishid 1, 1) PKG_BEGIN_TASK [1];
+      pkg_create (taskid 0) (finishid 1, 0) PKG_INIT []
+    ] in
+    let m := Map_FID.add (finishid 1) (0, [pkg_create (taskid 0) (finishid 1, 1) PKG_BEGIN_TASK [1]]) (Map_FID.empty _) in
+    buffer_add_all l (Map_FID.empty _) = ([
+      pkg_create (taskid 0) (finishid 1, 0) PKG_INIT [];
+      pkg_create (taskid 0) (finishid 1, 1) PKG_BEGIN_TASK [1]
+    ], Map_FID.add (finishid 1) (2, []) m).
+  Proof.
+    compute.
+    auto.
+  Qed.
+
   (** Regression test: *)
   Goal
     let foo := [
@@ -306,13 +468,17 @@ Section Defs.
    trivial.
   Qed.
 
-  Fixpoint parse_trace (l:list package) : option (list action) :=
+  Inductive parse_trace_err :=
+  PARSE_TRACE_ERR: nat -> pkg_parse_err -> parse_trace_err.
+
+  Fixpoint parse_trace (l:list package) : (list action + parse_trace_err) :=
   match l with
-  | [] => Some []
+  | [] => inl []
   | p::l =>
-    match pkg_parse_op p, parse_trace l with
-    | Some o, Some l => Some ((pkg_task p, o)::l)
-    | _, _ => None
+    match pkg_parse p, parse_trace l with
+    | inl o, inl l => inl ((pkg_task p, o)::l)
+    | _, inr e => inr e
+    | inr e, _ => inr (PARSE_TRACE_ERR (length l) e)
     end
   end.
 
@@ -325,7 +491,7 @@ Section Defs.
       pkg_create (taskid 2) (finishid 3, 0) PKG_BEGIN_FINISH [];
       pkg_create (taskid 2) (finishid 3, 1) PKG_BEGIN_TASK [5]
     ] in
-    parse_trace l = Some [
+    parse_trace l = inl [
       (taskid 0, INIT (finishid 1));
       (taskid 0, BEGIN_TASK (taskid 1));
       (taskid 1, BEGIN_FINISH (finishid 2));
@@ -338,28 +504,88 @@ Section Defs.
    trivial.
   Qed.
 
-  Fixpoint reduces_n (s:state) (l:list action): (state + reduces_err) % type :=
+  Inductive reduces_n_err :=
+  | REDUCES_N_ERROR: nat -> reduces_err -> reduces_n_err.
+
+  Fixpoint reduces_n (s:state) (l:list action): (state + reduces_n_err) % type :=
   match l with
   | [] => inl s
   | a::l =>
     match reduces s (fst a) (snd a) with
     | inl s =>
       reduces_n s l
-    | inr e => inr e
+    | inr e => inr (REDUCES_N_ERROR (length l) e)
     end
   end.
 
-  Let checks_add_aux ps b s : (checks + run_err) %type :=
+  Goal
+    let l := [
+      (taskid 0, INIT (finishid 0));
+      (taskid 0, INIT (finishid 1))
+    ] in
+    reduces_n (Map_TID.empty _) l = inr (REDUCES_N_ERROR 0 (TASK_EXIST (taskid 0))).
+  Proof.
+    intros.
+    simpl.
+    destruct (in_dec (finishid 0) (Map_TID.empty _)). {
+      apply not_in_empty in i.
+      contradiction.
+    }
+    remember (Map_TID.add _ _ _) as m.
+    destruct (in_dec (finishid 1) m). {
+      subst.
+      inversion i. {
+        inversion H; subst; clear H.
+        apply Map_TID_Facts.add_mapsto_iff in H0.
+        destruct H0 as [(?,Hx)|(?,?)]. {
+          subst.
+          inversion Hx; subst; clear Hx.
+        }
+        rewrite Map_TID_Facts.empty_mapsto_iff in *.
+        contradiction.
+      }
+      inversion H; subst; clear H.
+      rewrite Map_TID_Facts.add_mapsto_iff in *.
+      destruct H1 as [(?,Hx)|(?,?)]. {
+        subst.
+        inversion Hx; subst; clear Hx.
+        contradiction.
+      }
+      rewrite Map_TID_Facts.empty_mapsto_iff in *.
+      contradiction.
+    }
+    subst.
+    compute.
+    trivial.
+  Qed.
+
+  Inductive checks_err :=
+  | CHECKS_REDUCES_N_ERROR: package -> reduces_err -> checks_err
+  | CHECKS_INTERNAL_ERROR
+  | CHECKS_PARSE_TRACE_ERROR: parse_trace_err -> checks_err.
+
+  Fixpoint get {A} (n:nat) (l:list A) :=
+  match n, l with
+  | 0, [x] => Some x
+  | S n, x::l => get n l
+  | _, _ => None
+  end.
+
+  Let checks_add_aux ps b s : (checks + checks_err) %type :=
   match parse_trace ps with
-  | Some l =>
+  | inl l =>
     match reduces_n s l with
     | inl s => inl {| checks_buffer := b; checks_state := s |}
-    | inr e => inr (REDUCES_ERROR e)
+    | inr (REDUCES_N_ERROR n e) =>
+      match get n ps with
+      | Some p => inr (CHECKS_REDUCES_N_ERROR p e)
+      | None => inr CHECKS_INTERNAL_ERROR
+      end
     end
-  | None => inr (PKG_ERROR PARSE_ERROR)
+  | inr e => inr (CHECKS_PARSE_TRACE_ERROR e)
   end.
 
-  Definition checks_add (p:package) s : (checks + run_err) %type :=
+  Definition checks_add (p:package) s : (checks + checks_err) %type :=
   let (ps, b) := buffer_add p (checks_buffer s) in
   checks_add_aux ps b (checks_state s).
 
@@ -370,11 +596,8 @@ Section Defs.
 
   Definition count_enqueued s :=
     List.fold_left (fun accum y => accum + length (snd y)) (Map_FID_Extra.values (checks_buffer s)) 0.
-(*
-  Inductive load_err :=
-  | LOAD_ERROR: nat -> run_err -> load_err.
-*)
-  Definition checks_load (l:list package) : (checks + run_err) % type :=
+
+  Definition checks_load (l:list package) : (checks + checks_err) % type :=
   let (ps, b) := buffer_add_all l (Map_FID.empty _) in
   checks_add_aux ps b (Map_TID.empty _).
 End Defs.
@@ -412,4 +635,4 @@ Extract Inlined Constant eq_nat_dec => "( = )".
 Extraction Language Ocaml.
 
 Extraction "libhsem/lib/finish"
-  checks_add checks_make count_enqueued nat_to_op nat_to_args op_to_nat.
+  checks_add checks_make checks_load count_enqueued nat_to_op nat_to_args op_to_nat.
